Added linear sha256

benchmarks/lib/sha256.v
@@ -189,3 +189,92 @@ Qed.
 
 Definition SHA_256 (str : list byte) : list byte :=
     intlist_to_bytelist (hash_blocks init_registers (generate_and_pad str)).
+
+Require Import Lia.
+
+(* LINEAR-TIME FUNCTIONAL VERSION OF SHA256 *)
+Function zeros (n : Z) {measure Z.to_nat n} : list Int.int :=
+ if Z.gtb n 0 then Int.zero :: zeros (n-1) else nil.
+Proof.
+   intros. rewrite Z2Nat.inj_sub by lia.
+   apply Zgt_is_gt_bool in teq.
+   assert (0 < n) by lia. apply Z2Nat.inj_lt in H; try lia.
+Defined.
+
+Definition padlen (n: Z) : list Int.int :=
+    let p := n/4+3 (* number of words with trailing 128-byte,
+                                                      up to 3 zero bytes, and 2 length words *)
+    in let q := (p+15)/16*16 - p   (* number of zero-pad words *)
+      in zeros q ++ [Int.repr (n * 8 / Int.modulus); Int.repr (n * 8)].
+
+Fixpoint generate_and_pad' (n: list byte) len : list Int.int :=
+  match n with
+  | nil => bytes_to_Int (Byte.repr 128) Byte.zero Byte.zero Byte.zero :: padlen len
+  | [h1]=> bytes_to_Int h1 (Byte.repr 128) Byte.zero Byte.zero :: padlen (len+1)
+  | [h1; h2] => bytes_to_Int h1 h2 (Byte.repr 128) Byte.zero :: padlen (len+2)
+  | [h1; h2; h3] => bytes_to_Int h1 h2 h3 (Byte.repr 128) :: padlen (len+3)
+  | h1::h2::h3::h4::t => bytes_to_Int h1 h2 h3 h4 :: generate_and_pad' t (len+4)
+  end.
+
+Definition generate_and_pad_alt (n: list byte) : list Int.int :=
+   generate_and_pad' n 0.
+
+Definition Wnext (msg : list int) : int :=
+ match msg with
+ | x1::x2::x3::x4::x5::x6::x7::x8::x9::x10::x11::x12::x13::x14::x15::x16::_ =>
+   (Int.add (Int.add (sigma_1 x2) x7) (Int.add (sigma_0 x15) x16))
+ | _ => Int.zero  (* impossible *)
+ end.
+
+(*generating 64 words for the given message block imput*)
+Fixpoint generate_word (msg : list int) (n : nat) {struct n}: list int :=
+  match n with
+  |O   => msg
+  |S n' => generate_word (Wnext msg :: msg) n'
+  end.
+Arguments generate_word msg n : simpl never.
+Global Opaque generate_word. (* for some reason the Arguments...simpl-never
+   command does not do the job *)
+
+(*execute round function for 64 rounds*)
+Fixpoint rnd_64 (x: registers) (k w : list int) : registers :=
+  match k, w with
+  | k1::k', w1::w' => rnd_64 (rnd_function x k1 w1) k' w'
+  | _ , _ => x
+  end.
+Arguments rnd_64  x k w : simpl never.  (* blows up otherwise *)
+
+Definition process_block (r: registers) (block: list int) : registers :=
+       (map2 Int.add r (rnd_64 r K256 (rev(generate_word block 48)))).
+
+Fixpoint grab_and_process_block (n: nat) (r: registers) (firstrev msg: list int) : registers * list int :=
+ match n, msg with
+  | O, _ => (process_block r firstrev, msg)
+  | S n', m1::msg' => grab_and_process_block n' r (m1::firstrev) msg'
+  | _, nil => (r,nil) (* impossible *)
+ end.
+
+(*iterate through all the message blocks; this could have been done with just a Fixpoint
+  if we incorporated grab_and_process_block into process_msg, but I wanted to
+  modularize a bit more. *)
+Function process_msg  (r: registers) (msg : list int) {measure length msg}  : registers :=
+ match msg with
+ | nil => r
+ | _ => let (r', msg') := grab_and_process_block 16 r nil msg
+             in process_msg r' msg'
+ end.
+Proof.
+  intros; subst.
+  simpl.
+  assert (Datatypes.length msg' <= Datatypes.length l)%nat; [ | lia].
+  simpl in teq0.
+  do 16 (destruct l; [inv teq0; solve [simpl; auto 50] | ]).
+  unfold process_block in teq0.
+  assert (i15::l = msg') by congruence.
+  subst msg'.
+  simpl.
+  lia.
+Defined.
+
+Definition SHA_256' (str : list byte) : list byte :=
+    intlist_to_bytelist (process_msg init_registers (generate_and_pad_alt str)).
