benchmarks/tests.v
@@ -13,35 +13,34 @@ Import VeriStar.
 
 CertiCoq -help.
 
-(* Zoe : Currently not working *) 
-(* Definition test := "The message". *)
-(* Definition sha := sha256.SHA_256 (sha256.str_to_bytes test). *)
-
-(* CertiCoq Compile -ext "_cps" sha. *)
-(* CertiCoq Compile -direct demo1. *)
-(* CertiCoq Compile -O 2 -ext "_cps_opt" demo1. *)
-(* CertiCoq Compile -direct -O 2 -ext "_opt" demo1. *)
-
 Definition demo1 := List.app (List.repeat true 5) (List.repeat false 3).
 Definition demo2 := List.map negb [true; false; true].
 Definition demo3 := andb. 
 
 (* CertiCoq Show IR -debug -direct demo1. *)
 
+Eval compute in "Compiling demo1".
+
 CertiCoq Compile -ext "_cps" demo1.
 CertiCoq Compile -direct demo1.
 CertiCoq Compile -O 2 -ext "_cps_opt" demo1.
 CertiCoq Compile -direct -O 2 -ext "_opt" demo1.
+
+Eval compute in "Compiling demo2".
 
 CertiCoq Compile -ext "_cps" demo2.
 CertiCoq Compile -direct demo2.
 CertiCoq Compile -O 2 -ext "_cps_opt" demo2.
 CertiCoq Compile -direct -O 2 -ext "_opt" demo2.
 
+Eval compute in "Compiling demo3".
+
 CertiCoq Compile -ext "_cps" demo3.
 CertiCoq Compile -direct demo3.
 CertiCoq Compile -O 2 -ext "_cps_opt" demo3.
 CertiCoq Compile -direct -O 2 -ext "_opt" demo3.
+
+Eval compute in "Compiling list_sum".
 
 Definition list_sum := List.fold_left plus (List.repeat 1 100) 0.
 
@@ -65,10 +64,14 @@ Definition vs_hard :=
   | _ => false
   end.
 
+Eval compute in "Compiling vs_easy".
+
 CertiCoq Compile -direct -time vs_easy.
 CertiCoq Compile -ext "_cps" -time vs_easy.
 CertiCoq Compile -O 2 -ext "_cps_opt" vs_easy.
 CertiCoq Compile -direct -O 2 -ext "_opt" vs_easy.
+
+Eval compute in "Compiling vs_hard".
 
 CertiCoq Compile -ext "_cps" vs_hard.
 CertiCoq Compile -direct vs_hard.
@@ -77,6 +80,8 @@ CertiCoq Compile -direct -O 2 -ext "_opt" vs_hard.
 
 Definition binom := Binom.main.
 
+Eval compute in "Compiling binom".
+
 CertiCoq Compile -ext "_cps" binom. (* returns nat *)
 CertiCoq Compile -direct binom.  (* returns nat *)
 CertiCoq Compile -O 2 -ext "_cps_opt" binom.
@@ -84,7 +89,31 @@ CertiCoq Compile -direct -O 2 -ext "_opt" binom.
 
 Definition color := Color.main.
 
-CertiCoq Compile -ext "_cps" color.
-CertiCoq Compile -direct color.
-CertiCoq Compile -O 2 -ext "_cps_opt" color.
-CertiCoq Compile -direct -O 2 -ext "_opt" color.
+Eval compute in "Compiling color".
+
+CertiCoq Compile -time -ext "_cps" color.
+CertiCoq Compile -time -direct color.
+CertiCoq Compile -time -O 2 -ext "_cps_opt" color.
+CertiCoq Compile -time -direct -O 2 -ext "_opt" color.
+
+
+(* From the Coq website *)
+Definition test := "Coq is a formal proof management system. It provides a formal language to write mathematical definitions, executable algorithms and theorems together with an environment for semi-interactive development of machine-checked proofs. Typical applications include the certification of properties of programming languages (e.g. the CompCert compiler certification project, the Verified Software Toolchain for verification of C programs, or the Iris framework for concurrent separation logic), the formalization of mathematics (e.g. the full formalization of the Feit-Thompson theorem, or homotopy type theory), and teaching.".
+
+Definition sha := sha256.SHA_256 (sha256.str_to_bytes test).
+
+Definition sha_fast := sha256.SHA_256' (sha256.str_to_bytes test).
+
+Eval compute in "Compiling sha".
+
+CertiCoq Compile -ext "_cps" sha.
+CertiCoq Compile -direct sha.
+CertiCoq Compile -O 2 -ext "_cps_opt" sha.
+CertiCoq Compile -direct -O 2 -ext "_opt" sha.
+
+Eval compute in "Compiling sha_fast".
+
+CertiCoq Compile -ext "_cps" sha_fast.
+CertiCoq Compile -direct sha_fast.
+CertiCoq Compile -O 2 -ext "_cps_opt" sha_fast.
+CertiCoq Compile -direct -O 2 -ext "_opt" sha_fast.
